\documentclass[a4paper]{article}
\usepackage{mathtools}
\usepackage{amsmath}
\usepackage{amsthm}
\usepackage{amssymb}
\usepackage{framed}
\usepackage[makeroom]{cancel}
\usepackage{hyperref}

\newcommand{\pd}[3]{\left(\frac{\partial {#1}}{\partial {#2}}\right)_{#3}}
\newcommand{\pdd}[3]{\left(\frac{\partial^2 {#1}}{\partial {#2}\partial {#3}}\right)}

\title{Exercise sheet 3}
\author{Kai Keller}
\date{\today}

\begin{document}
\maketitle
\tableofcontents

\section{problem 1 - Einstein relations}
\paragraph{(a) compute:}
The fluctuation parameter matrix:
\begin{equation}
    \mathbf{g}=
    \begin{pmatrix}
        g_{UU} & g_{UV} \\
        g_{UV} & g_{VV}
    \end{pmatrix}
\end{equation}

and
\paragraph{(b) show:}
The following relations:
\begin{align}
    \pd{T}{V}{U}&=\frac{1}{C_V}\left( \frac{\alpha}{\kappa_T}T-p  \right) \\
    \pd{p}{V}{U}&=-\frac{1}{\kappa_TV}+\frac{\alpha}{\kappa_TC_V}\left( \frac{\alpha}{\kappa_T}T-p  \right)
    \label{second}
\end{align}

\paragraph{(a)}

To compute $g_{UU}$, we use the relation from the lecture:
\begin{align}
    g_{UU}&=-\pd{}{U}{V}\pd{}{U}{V} S(U,V) \\
          &=-\pd{}{U}{V}\pd{S}{U}{V} \\
          &=-\pd{}{U}{V}T^{-1} \\
          &=\frac{1}{T^2}\pd{T}{U}{V} \\
          &=\frac{1}{C_VT^2}
\end{align}
Where we used the differential of $S$:
\begin{align}
    dS&=\pd{S}{U}{V}dU+\pd{S}{U}{V}dV \\
    &=\frac{1}{T}dU+\frac{p}{T}dV
\end{align}
and the definition of the isochoric heat capacity $C_V=\pd{U}{T}{V}$.
We will proceed analog for the other cases:
\begin{align}
    g_{UV}&=-\pd{}{U}{V}\pd{}{V}{U}S \\
          &=-\pd{}{V}{U}\pd{S}{U}{V} \\
          &=\frac{1}{T^2}\pd{T}{V}{U} \\
          &=\frac{1}{T^2C_V}\left( \frac{\alpha}{\kappa_T}T-p  \right)
\end{align}
And finally
\begin{align}
    g_{VV}&=-\pd{}{V}{U}\pd{}{V}{U}S \\
          &=-\pd{}{V}{U}\pd{S}{V}{U} \\
          &=-\pd{}{V}{U}\frac{p}{T} \\
          &=-\frac{1}{T}\pd{p}{V}{U}+\frac{p}{T^2}\pd{T}{V}{U} \\
          &=\frac{1}{\kappa_TVT}-\frac{\alpha}{\kappa_TC_V}\left( \frac{\alpha}{\kappa_T}T-p  \right)+\frac{p}{T^2C_V}\left( \frac{\alpha}{\kappa_T}T-p  \right) \\
          &=\frac{1}{\kappa_TVT}+\frac{1}{C_V}\left( \frac{p}{T^2}-\frac{\alpha}{\kappa_T} \right)\left( \frac{\alpha}{\kappa_T}T-p  \right)
\end{align}

\paragraph{(b)}
We use the relation for $dU$ derived in exercise sheet 1, problem 1c (eq. 42):
\begin{equation}
    dU_{V,T}=\left( T\frac{\alpha}{\kappa_T}-p \right) dV + C_V dT \label{duvt}
\end{equation}
we want to find $\pd{T}{V}{U}$. From eq. \ref{duvt} we get for $dU=0$,
\begin{align}
     \left( \frac{\alpha}{\kappa_T}T-p  \right)dV&=C_V dT \\
      \Rightarrow \left. \frac{dT}{dV}\right|_{U=\text{const}}&=\pd{T}{V}{U}=\frac{1}{C_V}\left( \frac{\alpha}{\kappa_T}T-p  \right)
\end{align}
To show eq. \ref{second}, we use the relation $\pd{F}{V}{T}=-p$. With this we may write:
\begin{align}
    \pd{p}{V}{U}&=-\pd{}{V}{U}\pd{}{V}{T}F \\
    &=-\pd{}{V}{T}\pd{}{V}{U}U+\pd{}{V}{T}\pd{}{V}{U}(TS) \\
    &=\pd{}{V}{T}\left( S\pd{T}{V}{U}+T\pd{S}{V}{U}  \right) \\
    &=\pd{S}{V}{T}\pd{T}{V}{U}+\pd{p}{V}{T} \\
    &=\pd{p}{T}{V}\pd{T}{V}{U}+\pd{V}{p}{T}^{-1} \\
    &=\frac{\alpha}{\kappa_T}\frac{1}{C_V}\left(\frac{\alpha}{\kappa_T}T-p\right)-\frac{1}{V\kappa_T}
\end{align}

\end{document}


